refine the rel and thm statement

model/agp32RelationScript.sml
@@ -8,23 +8,31 @@ val _ = new_theory "agp32Relation";
     i: cycle (instr index) for the ISA.
  **)
 
+val _ = prefer_num ();
 val _ = guess_lengths ();
 
 (* Additional definitions for the pipeline correctness proofs *)
 (* enable_stg: stage k is enabled in the hardware circuit *)
-Definition enable_stg:
+Definition enable_stg_def:
   enable_stg k s =
-  if k = IF then s.IF.IF_PC_write_enable
-  else if k = ID then s.ID.ID_ID_write_enable
-  else if k = EX then s.ID.ID_EX_write_enable
-  else if k = MEM then (s.EX.EX_write_enable /\ s.MEM.MEM_state_flag) \/ s.MEM.MEM_enable
-  else (s.MEM.MEM_write_enable /\ s.WB.WB_state_flag) \/ s.WB.WB_enable
+  if k = 1 then s.IF.IF_PC_write_enable
+  else if k = 2 then s.ID.ID_ID_write_enable
+  else if k = 3 then s.ID.ID_EX_write_enable
+  else if k = 4 then (s.EX.EX_write_enable /\ s.MEM.MEM_state_flag) \/ s.MEM.MEM_enable
+  else if k = 5 then (s.MEM.MEM_write_enable /\ s.WB.WB_state_flag) \/ s.WB.WB_enable
+  else F
+End
+
+(* software conditions *)
+(* self modified: the instructions in IF, ID and EX stages do not fetch the address that MEM stage is writing *)
+Definition SC_self_mod_def:
+  SC_self_mod s <=> s.MEM.MEM_opc = 2w \/ s.MEM.MEM_opc = 3w ==> (s.PC <> s.data_addr) /\ (s.ID.ID_PC <> s.data_addr) /\ (s.EX.EX_PC <> s.data_addr)
 End
 
 
 (* Definitions of relations to prove the correctness of the pipelined Silver *)
 (* relation for the initial states *)
-Definition Init:
+Definition Init_def:
   Init (fext:ext) (s:state_circuit) (a:ag32_state) <=>
   (** CPU and ISA common items **)
   (s.PC = a.PC) /\
@@ -61,96 +69,96 @@ Definition Init:
 End
 
 (* relation between the pipelined Silver circuit and ISA state *)
-Definition Rel:
-  Rel (fext:ext) (s:state_circuit) (a:ag32_state) (k:pi_stg) (i:num) <=>
+Definition Rel_def:
+  Rel (fext:ext) (s:state_circuit) (k:num) (a:ag32_state) (i:num) <=>
+  fext.ready /\ (* to remove *)
   (fext.data_in = a.data_in) /\
   (** visible part: directly seen by ISA **)
   (** no visible registers in IF and ID **)
-  (k = EX ==>
+  (k = 3 ==>
    (s.EX.EX_carry_flag <=> (FUNPOW Next i a).CarryFlag) /\
    (s.EX.EX_overflow_flag <=> (FUNPOW Next i a).OverflowFlag) /\
-   (s.PC = (FUNPOW Next i a).PC)) /\
-  (k = MEM ==>
+   (s.EX.EX_jump_sel ==> s.PC = (FUNPOW Next i a).PC)) /\
+  (k = 4 ==>
    fext.mem = (FUNPOW Next i a).MEM) /\
-  (k = WB ==>
+  (k = 5 ==>
    (s.data_out = (FUNPOW Next i a).data_out) /\
    (s.R = (FUNPOW Next i a).R)) /\
   (** invisible part **)
-  (k = IF ==>
-   (s.IF.IF_instr = instr (FUNPOW Next i a))) /\
-  (k = ID ==>
+  (k = 1 ==>
+   (s.IF.IF_instr = instr (FUNPOW Next (i-1) a))) /\
+  (k = 2 ==>
    (s.ID.ID_PC = (FUNPOW Next (i-1) a).PC) /\
-   (s.ID.ID_instr = instr (FUNPOW Next i a)) /\
-   (** to correct **)
-   (s.ID.ID_addrA = addrA (FUNPOW Next i a)) /\
-   (s.ID.ID_addrB = addrB (FUNPOW Next i a)) /\
-   (s.ID.ID_addrW = addrW (FUNPOW Next i a)) /\
-   (s.ID.ID_addrA_disable <=> flagA (FUNPOW Next i a)) /\
-   (s.ID.ID_addrB_disable <=> flagB (FUNPOW Next i a)) /\
-   (s.ID.ID_addrW_disable <=> flagW (FUNPOW Next i a)) /\
-   (s.ID.ID_read_dataA_updated = reg_dataA (FUNPOW Next i a)) /\
-   (s.ID.ID_read_dataB_updated = reg_dataB (FUNPOW Next i a)) /\
-   (s.ID.ID_read_dataW_updated = reg_dataW (FUNPOW Next i a)) /\
-   (s.ID.ID_immA = immA (FUNPOW Next i a)) /\
-   (s.ID.ID_immB = immB (FUNPOW Next i a)) /\
-   (s.ID.ID_immW = immW (FUNPOW Next i a)) /\
-   (s.ID.ID_dataA = dataA (FUNPOW Next i a)) /\
-   (s.ID.ID_dataB = dataB (FUNPOW Next i a)) /\
-   (s.ID.ID_dataW = dataW (FUNPOW Next i a)) /\
-   (s.ID.ID_imm = imm (FUNPOW Next i a)) /\
-   (s.ID.ID_opc = opc (FUNPOW Next i a)) /\
-   (s.ID.ID_func = func (FUNPOW Next i a))) /\
-  (k = EX ==>
+   (s.ID.ID_instr = instr (FUNPOW Next (i - 1) a)) /\
+   (s.ID.ID_addrA = addrA (FUNPOW Next (i - 1) a)) /\
+   (s.ID.ID_addrB = addrB (FUNPOW Next (i - 1) a)) /\
+   (s.ID.ID_addrW = addrW (FUNPOW Next (i - 1) a)) /\
+   (s.ID.ID_addrA_disable <=> flagA (FUNPOW Next (i - 1) a)) /\
+   (s.ID.ID_addrB_disable <=> flagB (FUNPOW Next (i - 1) a)) /\
+   (s.ID.ID_addrW_disable <=> flagW (FUNPOW Next (i - 1) a)) /\
+   (s.ID.ID_read_dataA_updated = reg_dataA (FUNPOW Next (i - 1) a)) /\
+   (s.ID.ID_read_dataB_updated = reg_dataB (FUNPOW Next (i - 1) a)) /\
+   (s.ID.ID_read_dataW_updated = reg_dataW (FUNPOW Next (i - 1) a)) /\
+   (s.ID.ID_immA = immA (FUNPOW Next (i - 1) a)) /\
+   (s.ID.ID_immB = immB (FUNPOW Next (i - 1) a)) /\
+   (s.ID.ID_immW = immW (FUNPOW Next (i - 1) a)) /\
+   (s.ID.ID_dataA = dataA (FUNPOW Next (i - 1) a)) /\
+   (s.ID.ID_dataB = dataB (FUNPOW Next (i - 1) a)) /\
+   (s.ID.ID_dataW = dataW (FUNPOW Next (i - 1) a)) /\
+   (s.ID.ID_imm = imm (FUNPOW Next (i - 1) a)) /\
+   (s.ID.ID_opc = opc (FUNPOW Next (i - 1) a)) /\
+   (s.ID.ID_func = func (FUNPOW Next (i - 1) a))) /\
+  (k = 3 ==>
    (s.EX.EX_jump_sel ==> s.IF.IF_PC_input = (FUNPOW Next i a).PC) /\
-   (~s.EX.EX_jump_sel ==> s.IF.IF_PC_input = (FUNPOW Next i a).PC + 8w) /\
+   (~s.EX.EX_jump_sel ==> s.IF.IF_PC_input = (FUNPOW Next i a).PC + 4w) /\
    (s.EX.EX_PC = (FUNPOW Next (i-1) a).PC) /\
-   (s.EX.EX_addrA = addrA (FUNPOW Next i a)) /\
-   (s.EX.EX_addrB = addrB (FUNPOW Next i a)) /\
-   (s.EX.EX_addrW = addrW (FUNPOW Next i a)) /\
-   (s.EX.EX_addrA_disable <=> flagA (FUNPOW Next i a)) /\
-   (s.EX.EX_addrB_disable <=> flagB (FUNPOW Next i a)) /\
-   (s.EX.EX_addrW_disable <=> flagW (FUNPOW Next i a)) /\
-   (s.EX.EX_dataA_updated = dataA (FUNPOW Next i a)) /\
-   (s.EX.EX_dataB_updated = dataB (FUNPOW Next i a)) /\
-   (s.EX.EX_dataW_updated = dataW (FUNPOW Next i a)) /\
-   (s.EX.EX_dataA_rec = dataA (FUNPOW Next i a)) /\
-   (s.EX.EX_dataB_rec = dataB (FUNPOW Next i a)) /\
-   (s.EX.EX_dataW_rec = dataW (FUNPOW Next i a)) /\
-   (s.EX.EX_imm = imm (FUNPOW Next i a)) /\
-   (s.EX.EX_ALU_res = ALU_res (FUNPOW Next i a)) /\
-   (s.EX.EX_SHIFT_res = shift_res (FUNPOW Next i a)) /\
+   (s.EX.EX_addrA = addrA (FUNPOW Next (i-1) a)) /\
+   (s.EX.EX_addrB = addrB (FUNPOW Next (i-1) a)) /\
+   (s.EX.EX_addrW = addrW (FUNPOW Next (i-1) a)) /\
+   (s.EX.EX_addrA_disable <=> flagA (FUNPOW Next (i-1) a)) /\
+   (s.EX.EX_addrB_disable <=> flagB (FUNPOW Next (i-1) a)) /\
+   (s.EX.EX_addrW_disable <=> flagW (FUNPOW Next (i-1) a)) /\
+   (s.EX.EX_dataA_updated = dataA (FUNPOW Next (i-1) a)) /\
+   (s.EX.EX_dataB_updated = dataB (FUNPOW Next (i-1) a)) /\
+   (s.EX.EX_dataW_updated = dataW (FUNPOW Next (i-1) a)) /\
+   (s.EX.EX_dataA_rec = dataA (FUNPOW Next (i-1) a)) /\
+   (s.EX.EX_dataB_rec = dataB (FUNPOW Next (i-1) a)) /\
+   (s.EX.EX_dataW_rec = dataW (FUNPOW Next (i-1) a)) /\
+   (s.EX.EX_imm = imm (FUNPOW Next (i-1) a)) /\
+   (s.EX.EX_ALU_res = ALU_res (FUNPOW Next (i-1) a)) /\
+   (s.EX.EX_SHIFT_res = shift_res (FUNPOW Next (i-1) a)) /\
    (s.EX.EX_jump_sel ==> s.EX.EX_jump_addr = (FUNPOW Next i a).PC) /\
-   (s.EX.EX_opc = opc (FUNPOW Next i a)) /\
-   (s.EX.EX_func = func (FUNPOW Next i a))) /\
-  (k = MEM ==>
+   (s.EX.EX_opc = opc (FUNPOW Next (i-1) a)) /\
+   (s.EX.EX_func = func (FUNPOW Next (i-1) a))) /\
+  (k = 4 ==>
    (s.MEM.MEM_PC = (FUNPOW Next (i-1) a).PC) /\
-   (s.MEM.MEM_addrW = addrW (FUNPOW Next i a)) /\
-   (s.MEM.MEM_dataA = dataA (FUNPOW Next i a)) /\
-   (s.MEM.MEM_dataB = dataB (FUNPOW Next i a)) /\
-   (s.MEM.MEM_dataW = dataW (FUNPOW Next i a)) /\
-   (s.MEM.MEM_imm = imm (FUNPOW Next i a)) /\
+   (s.MEM.MEM_addrW = addrW (FUNPOW Next (i-1) a)) /\
+   (s.MEM.MEM_dataA = dataA (FUNPOW Next (i-1) a)) /\
+   (s.MEM.MEM_dataB = dataB (FUNPOW Next (i-1) a)) /\
+   (s.MEM.MEM_dataW = dataW (FUNPOW Next (i-1) a)) /\
+   (s.MEM.MEM_imm = imm (FUNPOW Next (i-1) a)) /\
    (s.MEM.MEM_imm_updated =
-    ((8 >< 0) (imm (FUNPOW Next i a))) @@ ((22 >< 0) (dataW (FUNPOW Next i a)))) /\
-   (s.MEM.MEM_ALU_res = ALU_res (FUNPOW Next i a)) /\
-   (s.MEM.MEM_SHIFT_res = shift_res (FUNPOW Next i a)) /\
-   (s.MEM.MEM_write_reg <=> reg_ifwrite (FUNPOW Next i a)) /\
-   (s.MEM.MEM_opc = opc (FUNPOW Next i a)) /\
-   (s.data_addr = mem_data_addr (FUNPOW Next i a)) /\
-   (s.data_wstrb = mem_data_wstrb (FUNPOW Next i a)) /\
-   (s.data_wdata = mem_data_wdata (FUNPOW Next i a)) /\
-   (fext.data_rdata = mem_data_rdata (FUNPOW Next i a))) /\
-  (k = WB ==>
+    ((8 >< 0) (imm (FUNPOW Next (i-1) a))) @@ ((22 >< 0) (dataW (FUNPOW Next (i-1) a)))) /\
+   (s.MEM.MEM_ALU_res = ALU_res (FUNPOW Next (i-1) a)) /\
+   (s.MEM.MEM_SHIFT_res = shift_res (FUNPOW Next (i-1) a)) /\
+   (s.MEM.MEM_write_reg <=> reg_ifwrite (FUNPOW Next (i-1) a)) /\
+   (s.MEM.MEM_opc = opc (FUNPOW Next (i-1) a)) /\
+   (s.data_addr = mem_data_addr (FUNPOW Next (i-1) a)) /\
+   (s.data_wstrb = mem_data_wstrb (FUNPOW Next (i-1) a)) /\
+   (s.data_wdata = mem_data_wdata (FUNPOW Next (i-1) a)) /\
+   (fext.data_rdata = mem_data_rdata (FUNPOW Next (i-1) a))) /\
+  (k = 5 ==>
    (s.WB.WB_PC = (FUNPOW Next (i-1) a).PC) /\
-   (s.WB.WB_addrW = addrW (FUNPOW Next i a)) /\
-   (s.WB.WB_dataA = dataA (FUNPOW Next i a)) /\
+   (s.WB.WB_addrW = addrW (FUNPOW Next (i-1) a)) /\
+   (s.WB.WB_dataA = dataA (FUNPOW Next (i-1) a)) /\
    (s.WB.WB_opc = 14w ==> s.WB.WB_imm =
-                          ((8 >< 0) (imm (FUNPOW Next i a))) @@ ((22 >< 0) (dataW (FUNPOW Next i a)))) /\
-   (s.WB.WB_opc <> 14w ==> s.WB.WB_imm = imm (FUNPOW Next i a)) /\
-   (s.WB.WB_ALU_res = ALU_res (FUNPOW Next i a)) /\
-   (s.WB.WB_SHIFT_res = shift_res (FUNPOW Next i a)) /\
-   (s.WB.WB_write_reg = reg_ifwrite (FUNPOW Next i a)) /\
-   (s.WB.WB_opc = opc (FUNPOW Next i a)) /\
-   (s.WB.WB_write_data = reg_wdata (FUNPOW Next i a)))
+                          ((8 >< 0) (imm (FUNPOW Next (i-1) a))) @@ ((22 >< 0) (dataW (FUNPOW Next (i-1) a)))) /\
+   (s.WB.WB_opc <> 14w ==> s.WB.WB_imm = imm (FUNPOW Next (i-1) a)) /\
+   (s.WB.WB_ALU_res = ALU_res (FUNPOW Next (i-1) a)) /\
+   (s.WB.WB_SHIFT_res = shift_res (FUNPOW Next (i-1) a)) /\
+   (s.WB.WB_write_reg = reg_ifwrite (FUNPOW Next (i-1) a)) /\
+   (s.WB.WB_opc = opc (FUNPOW Next (i-1) a)) /\
+   (s.WB.WB_write_data = reg_wdata (FUNPOW Next (i-1) a)))
 End
 
 val _ = export_theory ();
