proof/agp32CorrectScript.sml
@@ -1,0 +1,29 @@
+open hardwarePreamble agp32StateTheory agp32EnvironmentTheory agp32ProcessorTheory ag32Theory ag32ExtraTheory agp32RelationTheory;
+
+val _ = new_theory "agp32Correct";
+
+val _ = prefer_num ();
+val _ = guess_lengths ();
+
+(* I: scheduling function
+   C: cache oracle
+ *)
+Theorem agp32_Rel_ag32_correct:
+  !(k:num) fext fbits s a (t:num) i I C.
+    s = agp32 fext fbits ==>
+    SC_self_mod (s t) ==>
+    is_mem fext_accessor_circuit s fext ==>
+    is_acc accelerator_f s ==>
+    is_interrupt_interface fext_accessor_circuit s fext ==>
+    (* cache oracle can introduce hit/miss *)
+    (C (s t).data_addr (s t).data_wstrb (s t).data_wdata (s t).command (s t).PC <=> (fext t).ready) ==>
+    Init (fext 0) (s 0) a ==>
+    (** properties of scheduling function I **)
+    (enable_stg k (s t) ==> I(k,t) = I(k-1,t) - 1) ==>
+    I(k,t) = i ==>
+    Rel (fext t) (s t) k a i
+Proof
+  REPEAT STRIP_TAC >> cheat
+QED
+
+val _ = export_theory ();
